@base             <http://w3id.org/oseg/ont/okh-krawler> .
@prefix okhkrawl: <#> .
@prefix dcat:     <http://www.w3.org/ns/dcat#> .
@prefix dcterms:  <http://purl.org/dc/terms/> .
@prefix foaf:     <http://xmlns.com/foaf/0.1/> .
@prefix orcid:    <http://orcid.org/> .
@prefix osegprof: <http://w3id.org/oseg/ont/oseg-profiles#> .
@prefix rdf:      <http://www.w3.org/1999/02/22-rdf-syntax-ns#> .
@prefix rdfs:     <http://www.w3.org/2000/01/rdf-schema#> .
@prefix schema:   <http://schema.org/> .
@prefix skos:     <http://www.w3.org/2004/02/skos/core#> .
@prefix spdx:     <http://spdx.org/rdf/terms#> .
@prefix spdxl:    <http://spdx.org/licenses/> .
@prefix vaem:     <http://www.linkedmodel.org/schema/vaem#> .




okh:created
  a owl:ObjectProperty ;
  a skos:Concept ;
  rdfs:label "data creation time-stamp"@en ;
  rdfs:comment "Date and time of the creation of this meta-data, following ISO 8601; see: <https://www.w3.org/TR/xmlschema11-2/#dateTimeStamp>"@en ;
  rdfs:subPropertyOf dcterms:created ;
  vs:term_status "unstable" ;
  schema:domainIncludes okh:Dataset ;
  schema:rangeIncludes okh:TimeStamp ;
  okhmeta:hasMetaTag okhmeta:DataGatheringTag ;
  .

#   okh:lastChanged "2021-03-26T15:15:46+00:00" ;
#   okh:lastVisited "2021-03-26T15:15:46+00:00" ;



okhkrawl:okhKrawlerDataset
  a dcat:Dataset ;
  rdfs:label "OKH Krawler Dataset" ;
  okh:dataProvider <> ;
  void:sparqlEndpoint <http://okh.dev.opensourceecology.de/sparql>;
  spdx:licenseDeclared spdxl:ODbL-1.0 ;
  skos:editorialNote '''
# SPDX-FileCopyrightText: Robin Vobruba <hoijui.quaero@gmail.com>
# SPDX-License-Identifier: ODbL-1.0
''' ;
  dcterms:creator osegprof:robinVobruba ;
  okh:organization osegprof:osegAssociation ;
  dcterms:description "The OKH triples specific to crawling OHS projects with the Krawler software"@en ;
  dcterms:identifier <> ;
  dcat:distribution okhkrawl:okhKrawlerDataset-ttl ;
  .

okhkrawl:okhKrawlerDataset-ttl
  a dcat:Distribution ;
  rdfs:label "OKH Krawler Dataset Distribution" ;
  dcat:downloadURL <> ;
  dcat:mediaType <http://www.iana.org/assignments/media-types/text/turtle> ;
  .

okhkrawl:dataProviderAppropedia
  a okh:DataProvider ;
  rdfs:label "Appropedia" ;
  dcterms:title "Appropedia" ;
  dcterms:identifier "https://appropedia.org"^^xsd:anyURI ;
  .

okhkrawl:dataProviderCodeberg
  a okh:DataProvider ;
  rdfs:label "CodeBerg" ;
  dcterms:title "CodeBerg" ;
  dcterms:identifier "https://codeberg.org"^^xsd:anyURI ;
  .

okhkrawl:dataProviderGithub
  a okh:DataProvider ;
  rdfs:label "GitHub" ;
  dcterms:title "GitHub" ;
  dcterms:identifier "https://github.com"^^xsd:anyURI ;
  .

okhkrawl:dataProviderGitlab
  a okh:DataProvider ;
  rdfs:label "GitLab.com" ;
  dcterms:title "GitLab.com" ;
  dcterms:identifier "https://gitlab.com"^^xsd:anyURI ;
  .

okhkrawl:dataProviderGitlabOpenSourceEcologyGermany
  a okh:DataProvider ;
  rdfs:label "gitlab@OSEG" ;
  dcterms:title "gitlab@OSEG" ;
  dcterms:identifier "https://gitlab.opensourceecology.de"^^xsd:anyURI ;
  .

okhkrawl:dataProviderOshwa
  a okh:DataProvider ;
  rdfs:label "OSHWA" ;
  dcterms:title "OSHWA" ;
  dcterms:identifier "certification.oshwa.org"^^xsd:anyURI ;
  .

okhkrawl:dataProviderThingiverse
  a okh:DataProvider ;
  rdfs:label "Thingiverse" ;
  dcterms:title "Thingiverse" ;
  dcterms:identifier "https://www.thingiverse.com"^^xsd:anyURI ;
  .

okhkrawl:dataSourcingProcedureApi
  a okh:DataSourcingProcedure ;
  rdfs:label "API" ;
  dcterms:title "API" ;
  rdfs:comment "The API of the platform hosting the project is crawled to create a manifest, which is then converted to (OKH) RDF triples" ;
  .

okhkrawl:dataSourcingProcedureGeneratedManifest
  a okh:DataSourcingProcedure ;
  rdfs:label "Generated Manifest" ;
  dcterms:title "Generated Manifest" ;
  rdfs:comment "The platform hosting the project generates a manifest, which is then crawled and converted to (OKH) RDF triples" ;
  .

okhkrawl:dataSourcingProcedureManifest
  a okh:DataSourcingProcedure ;
  rdfs:label "Manifest" ;
  dcterms:title "Manifest" ;
  rdfs:comment "The project supplies a manifest, which is then crawled and converted to (OKH) RDF triples" ;
  .

okhkrawl:dataSourcingProcedureDirect
  a okh:DataSourcingProcedure ;
  rdfs:label "Direct" ;
  dcterms:title "Direct" ;
  rdfs:comment "The project directly supplies (OKH) RDF triples, which are then crawled" ;
  .
